more cleanup

LeanStlc/StrongNorm.lean
@@ -28,7 +28,7 @@ namespace StrongNormalizaton
     intro j; induction A generalizing Γ t
     all_goals simp at j; grind
 
-  theorem LR.monotone (m : Γ -⟨r⟩> Δ) : LR Γ A t -> LR Δ A (t[r]) := by
+  theorem LR.monotone (m : Γ -⟨r⟩> Δ) : LR Γ A t -> LR Δ A t[r] := by
     intro h; induction A generalizing Γ Δ t r
     case arrow A B ih1 ih2 =>
       apply And.intro
@@ -46,49 +46,50 @@ namespace StrongNormalizaton
     replace h1 := h1 h2
     apply LR.typing h1
 
-  theorem cr :
-    (∀ {Γ t}, LR Γ A t -> SnNor t)
-    ∧ (∀ {Γ t}, Γ ⊢ t : A -> SnNeu t -> LR Γ A t)
-    ∧ (∀ {Γ t t'}, Γ ⊢ t : A -> SnRed t t' -> LR Γ A t' -> LR Γ A t)
-  := by
-    induction A <;> simp at *
-    case arrow A B ih1 ih2 =>
-      apply And.intro
-      case _ =>
-        intro Γ t j h
-        apply @SnNor.antirename (t[Ren.to (· + 1)]) (· + 1) _ t rfl
-        apply @SnNor.beta_var _ _ _ 0 rfl
-        replace h := h TypingRen.succ (@ih1.2.1 (A::Γ) #0 (.var (by simp)) .var)
-        simp at h
-        apply ih2.1 h
-      case _ =>
-        apply And.intro
-        case _ =>
-          intro Γ t j h
-          apply And.intro j
-          intro r Δ v m lv
-          apply ih2.2.1
-          apply Typing.app _ (LR.typing lv); apply Typing.rename m j
-          apply SnNeu.app
-          apply SnNeu.rename r h
-          apply ih1.1 lv
-        case _ =>
-          intro Γ t t' j1 h1 j2 h2
-          apply And.intro j1
-          intro r Δ v m lv
-          have lem1 := h2 m lv
-          apply @ih2.2.2 _ (t[r] :@ v) (t'[r] :@ v) _ _ lem1
-          apply Typing.app _ (LR.typing lv); apply Typing.rename m j1
-          replace h1 := SnRed.rename r h1; simp at h1
-          apply SnRed.step_app h1
-    all_goals
-      apply And.intro; grind
-      intro Γ t t' j1 h1 j2 h2
-      apply And.intro j1
-      apply SnNor.red h1 h2
+  mutual
+    def cr1 : ∀ {A}, LR Γ A t -> SnNor t
+    | .base, ⟨j1, j2⟩ => j2
+    | .nat, ⟨j1, j2⟩ => j2
+    | .arrow A B, ⟨j1, j2⟩ =>
+      let j2'  : LR (A::Γ) B (t[+1] :@ #0) := j2 TypingRen.succ $ cr2 (.var $ by simp) .var
+      let lem1 : SnNor t[+1]               := SnNor.beta_var (cr1 j2') rfl
+      SnNor.antirename (· + 1) lem1 t rfl
+
+    def cr2 : ∀ {A}, Γ ⊢ t : A -> SnNeu t -> LR Γ A t
+    | .base, j1, j2 => ⟨j1, .neu j2⟩
+    | .nat, j1, j2 => ⟨j1, .neu j2⟩
+    | .arrow A B, j, j2 =>
+      let lem {r Δ v} (m : Γ -⟨r⟩> Δ) (lv : LR Δ A v) : LR Δ B (t[r.to] :@ v) :=
+        let lem1 : Δ ⊢ (t[r] :@ v) : B := .app (j.rename m) lv.typing
+        let lem2 : SnNeu (t[r] :@ v)   := .app (j2.rename r) (cr1 lv)
+        cr2 lem1 lem2
+      ⟨j, lem⟩
+
+    def cr3 : ∀ {A}, Γ ⊢ t : A -> SnRed t t' -> LR Γ A t' -> LR Γ A t
+    | .base, j, r, ⟨_, h2⟩ => ⟨j, .red r h2⟩
+    | .nat, j, r, ⟨_, h2⟩ => ⟨j, .red r h2⟩
+    | .arrow A B, j, sr, tl =>
+      let lem {r Δ v} (m : Γ -⟨r⟩> Δ) (lv : LR Δ A v) : LR Δ B (t[r.to] :@ v) :=
+        have lem1 : Δ ⊢ (t[r] :@ v) : B            := .app (j.rename m) lv.typing
+        have lem2 : SnRed (t[r] :@ v) (t'[r] :@ v) := SnRed.step_app (sr.rename r)
+        cr3 lem1 lem2 (tl.2 m lv)
+      ⟨j, lem⟩
+  end
 
   theorem LR.var {A x} : Γ ⊢ #x : A -> LR Γ A #x := by
-    intro j; apply cr.2.1 j; apply SnNeu.var
+    intro j; apply cr2 j; apply SnNeu.var
+
+  theorem GR.from_ren (m : Γ -⟨r⟩> Δ) : GR Γ Δ r.to
+  | _, _, h => LR.var $ .var (m h)
+
+  theorem GR.compose {r : Ren} (a : GR X Y σ) (b : GR Y Z r.to) : GR X Z (σ ∘ r.to)
+  | x, T, h =>
+    let m : Y -⟨r⟩> Z := TypingSubst.forget b.forget
+    cast (by simp) $ LR.monotone m (a h)
+
+  theorem GR.su (j : LR Δ A a) (m : GR Γ Δ σ) : GR (A::Γ) Δ (su a::σ)
+  | 0, T, h => cast (by simp; grind) j
+  | x + 1, T, h => m h
 
   theorem LR.nrec_neutral
     (h1 : LR Γ A z)
@@ -98,47 +99,42 @@ namespace StrongNormalizaton
     : LR Γ A (.nrec A z s n)
   :=
     let lem := Typing.nrec (LR.typing h1) (LR.typing h2) h3
-    cr.2.1 lem (SnNeu.nrec (cr.1 h1) (cr.1 h2) h4)
+    cr2 lem (SnNeu.nrec (cr1 h1) (cr1 h2) h4)
 
   theorem LR.app (flr : LR Γ (A -t> B) f) (alr : LR Γ A a) : LR Γ B (f :@ a) :=
-    let lem := flr.2 TypingRen.id alr
-    by simp at lem; exact lem
+    cast (by simp) $ flr.2 TypingRen.id alr
 
   def LR.nrec (h1 : LR Γ A z) (h2 : LR Γ (A -t> A) s) (j : Γ ⊢ n : Ty.nat)
     : SnNor n -> LR Γ A (.nrec A z s n)
   | .lam t => by cases j
   | .zero =>
     let j' := (Typing.nrec (LR.typing h1) (LR.typing h2) j)
-    cr.2.2 j' (SnRed.zero (cr.1 h2)) h1
+    cr3 j' (SnRed.zero (cr1 h2)) h1
   | .succ t =>
     let j' := (Typing.nrec (LR.typing h1) (LR.typing h2) j)
-    cr.2.2 j' SnRed.succ (app h2 (nrec h1 h2 (by cases j; grind) t))
+    cr3 j' SnRed.succ (app h2 (nrec h1 h2 (by cases j; grind) t))
   | .neu t => nrec_neutral h1 h2 j t
   | .red r t' =>
     let j' := (Typing.nrec (LR.typing h1) (LR.typing h2) j)
     let r' := SnRed.weaken r
-    cr.2.2 j' (SnRed.step_nrec r) (LR.nrec h1 h2 (j.preservation_step r') t')
+    cr3 j' (SnRed.step_nrec r) (LR.nrec h1 h2 (j.preservation_step r') t')
 
   def fundamental : Γ ⊢ t : A -> Γ ⊨s t : A
   | .var j, σ, Δ, h => h j
-  | .app fj aj, σ, Δ, h =>
+  | .app (f := f) (a := a) fj aj, σ, Δ, h =>
     let aj' := fundamental aj σ Δ h
-    let fj' := (fundamental fj σ Δ h).2 TypingRen.id aj'
-    by simp at fj'; exact fj'
+    let fj' : LR Δ A (f[σ] :@ a[σ]) := cast (by simp) $ (fundamental fj σ Δ h).2 TypingRen.id aj'
+    fj'
   | @Typing.lam _ A B t tj, σ, Δ, h =>
     let m1 : Γ -[σ]> Δ := h.forget
     let lem1 := .subst m1 (.lam tj)
     let lem2 {r Δ' v} (m2 : Δ -⟨r⟩> Δ') (lv : LR Δ' A v) : LR Δ' B ((:λ[A] t)[σ][r] :@ v) :=
-      let tj' := fundamental tj (.su v::σ ∘ r.to) Δ' (by {
-        intro x T h2; cases x <;> simp at *
-        subst h2; exact lv
-        have lem := LR.monotone m2 (h h2)
-        simp at lem; exact lem
-      })
-      let lem2 := @SnRed.beta v A (t[.re 0::σ ∘ r ∘ +1]) (cr.1 lv)
-      @cr.2.2 _ _ (t[.su v::σ ∘ r.to])
+      let m3  : GR (A :: Γ) Δ' (su v::σ ∘ r.to) := GR.su lv $ h.compose (GR.from_ren m2)
+      let tj' : LR Δ' B t[su v::σ ∘ r.to]       := fundamental tj (.su v::σ ∘ r.to) Δ' m3
+      let lem2 := @SnRed.beta v A (t[.re 0::σ ∘ r ∘ +1]) (cr1 lv)
+      @cr3 _ _ (t[.su v::σ ∘ r.to]) _
         (.app (.rename m2 lem1) (LR.typing lv))
-        (by simp at lem2; simp; exact lem2)
+        (cast (by simp) $ lem2)
         tj'
     ⟨lem1, lem2⟩
   | .zero, σ, Δ, h => ⟨.zero, .zero⟩
@@ -148,69 +144,6 @@ namespace StrongNormalizaton
   | .nrec zj sj nj, σ, Δ, h =>
     let ⟨ih1, ih2⟩ := fundamental nj σ Δ h
     LR.nrec (fundamental zj σ Δ h) (fundamental sj σ Δ h) ih1 ih2
-
-  -- theorem fundamental2 {Γ t A} : Γ ⊢ t : A -> Γ ⊨s t : A := by
-  --   intro j; induction j
-  --   case var Γ T x j =>
-  --     simp; intro σ Δ h
-  --     apply h j
-  --   case app Γ A B f a j1 j2 ih1 ih2 =>
-  --     simp; intro σ Δ h; simp at ih1
-  --     replace ih2 := ih2 σ Δ h
-  --     replace ih1 := (ih1 σ Δ h).2 TypingRen.id ih2
-  --     simp at ih1; apply ih1
-  --   case lam Γ A B t j ih =>
-  --     simp; intro σ Δ h; apply And.intro
-  --     apply Typing.lam
-  --     have lem : Γ -[σ]> Δ := GR.forget h
-  --     replace lem : A::Γ -[σ.lift]> A::Δ := TypingSubst.lift A lem
-  --     simp at lem; apply Typing.subst lem j
-  --     intro r Δ' v m lv
-  --     have lem : t[.re 0::σ ∘ r ∘ +1][.su v :: +0] = t[.su v::σ ∘ r.to] := by simp
-  --     apply @cr.2.2 _ _ (t[.su v::σ ∘ r.to])
-  --     apply Typing.app _ (LR.typing lv); apply Typing.lam
-  --     have lem3 := Typing.subst (TypingSubst.lift _ (GR.forget h)) j
-  --     replace lem3 := Typing.rename (TypingRen.lift _ m) lem3
-  --     rw [Ren.to_lift] at lem3; simp at lem3; apply lem3
-  --     have lem2 := @SnRed.beta v A (t[.re 0::σ ∘ r ∘ +1]); simp at lem2
-  --     apply lem2
-  --     apply cr.1 lv
-  --     replace ih := ih (.su v :: σ ∘ r.to) Δ'
-  --     apply ih
-  --     simp; intro x T j2
-  --     cases x
-  --     case _ =>
-  --       simp; simp at j2; subst j2
-  --       apply lv
-  --     case _ x =>
-  --       simp; simp at j2
-  --       replace h := h j2
-  --       unfold Subst.compose; simp
-  --       generalize zdef : σ x = z at *
-  --       cases z <;> simp at *
-  --       case _ k =>
-  --         have lem := LR.monotone m h; simp at lem
-  --         generalize wdef : r k = w at *
-  --         cases w <;> simp [*]
-  --       case _ t => apply LR.monotone m h
-  --   case zero =>
-  --     intro σ Δ h; simp
-  --     apply And.intro; apply Typing.zero
-  --     apply SnNor.zero
-  --   case succ Γ n j ih =>
-  --     intro σ Δ h; simp
-  --     replace ih := ih σ Δ h; simp at ih
-  --     apply And.intro
-  --     apply Typing.succ ih.1
-  --     apply SnNor.succ ih.2
-  --   case nrec Γ z A s n j1 j2 j3 ih1 ih2 ih3 =>
-  --     intro σ Δ h; simp
-  --     replace ih1 := ih1 σ Δ h
-  --     replace ih2 := ih2 σ Δ h
-  --     replace ih3 := ih3 σ Δ h
-  --     have lem2 := Typing.subst (GR.forget h) j3
-  --     apply LR.nrec ih1 ih2 lem2
-  --     apply cr.1 ih3
 end StrongNormalizaton
 
 theorem strong_normalization_inductive (j : Γ ⊢ t : A) : SnNor t :=
@@ -218,8 +151,9 @@ theorem strong_normalization_inductive (j : Γ ⊢ t : A) : SnNor t :=
     simp; intro x T h
     apply StrongNormalizaton.LR.var
     apply Typing.var h
-  let lem2 := StrongNormalizaton.fundamental j +0 Γ lem1
-  StrongNormalizaton.cr.1 (by simp at lem2; exact lem2)
+  let lem2 : StrongNormalizaton.LR Γ A t :=
+    cast (by simp) $ StrongNormalizaton.fundamental j +0 Γ lem1
+  StrongNormalizaton.cr1 lem2
 
 theorem strong_normalization (j : Γ ⊢ t : A) : SN Red t :=
   SnNor.sound $ strong_normalization_inductive j
